genperm_Type.v
@@ -1,20 +1,19 @@
-(* genperm_Type Library *)
-
 (** * Factorized statements for different notions of permutation *)
 
 Require Import List CMorphisms.
 Require Import funtheory Permutation_Type_more Permutation_Type_solve CPermutation_Type CPermutation_Type_solve.
 
+Set Implicit Arguments.
 
 (** ** Definitions
  parametrized by a boolean. *)
 
 (** Permutation or cyclic permutation *)
-Definition PCperm_Type {A} (b : bool) :=
+Definition PCperm_Type A (b : bool) :=
   if b then @Permutation_Type A else @CPermutation_Type A.
 
 (** Permutation or equality *)
-Definition PEperm_Type {A} (b : bool) :=
+Definition PEperm_Type A (b : bool) :=
   if b then @Permutation_Type A else @eq (list A).
 
 
@@ -40,19 +39,19 @@ Ltac PCperm_Type_solve :=
 
 (** *** Properties *)
 
-Instance PCperm_perm_Type {A} b : Proper (PCperm_Type b ==> (@Permutation_Type A)) id.
+Instance PCperm_perm_Type A b : Proper (PCperm_Type b ==> (@Permutation_Type A)) id.
 Proof with try assumption.
 destruct b ; intros l l' HP...
 apply cperm_perm_Type...
 Qed.
 
-Instance cperm_PCperm_Type {A} b : Proper (CPermutation_Type ==> PCperm_Type b) (@id (list A)).
+Instance cperm_PCperm_Type A b : Proper (CPermutation_Type ==> PCperm_Type b) (@id (list A)).
 Proof with try assumption.
 destruct b ; intros l l' HC...
 apply cperm_perm_Type...
 Qed.
 
-Lemma PCperm_Type_monot {A} : forall b1 b2, Bool.leb b1 b2 ->
+Lemma PCperm_Type_monot A : forall b1 b2, Bool.leb b1 b2 ->
   forall l1 l2 : list A, PCperm_Type b1 l1 l2 -> PCperm_Type b2 l1 l2.
 Proof.
 intros b1 b2 Hleb l1 l2.
@@ -60,28 +59,28 @@ destruct b1; destruct b2; try (now inversion Hleb).
 apply cperm_perm_Type.
 Qed.
 
-Instance PCperm_Type_refl {A} b : Reflexive (@PCperm_Type A b).
+Instance PCperm_Type_refl A b : Reflexive (@PCperm_Type A b).
 Proof.
 destruct b ; intros l.
 - apply Permutation_Type_refl.
 - apply cperm_Type_refl.
 Qed.
 
-Instance PCperm_Type_sym {A} b : Symmetric (@PCperm_Type A b).
+Instance PCperm_Type_sym A b : Symmetric (@PCperm_Type A b).
 Proof with try assumption.
 destruct b ; intros l l' H.
 - apply Permutation_Type_sym...
 - apply cperm_Type_sym...
 Qed.
 
-Instance PCperm_Type_trans {A} b : Transitive (@PCperm_Type A b).
+Instance PCperm_Type_trans A b : Transitive (@PCperm_Type A b).
 Proof with try eassumption.
 destruct b ; intros l l' l'' H1 H2.
 - eapply Permutation_Type_trans...
 - eapply cperm_Type_trans...
 Qed.
 
-Instance PCperm_Type_equiv {A} b : Equivalence (@PCperm_Type A b).
+Instance PCperm_Type_equiv A b : Equivalence (@PCperm_Type A b).
 Proof.
 split.
 - apply PCperm_Type_refl.
@@ -89,7 +88,7 @@ split.
 - apply PCperm_Type_trans.
 Qed.
 
-Lemma PCperm_Type_swap {A} b : forall a1 a2 : A,
+Lemma PCperm_Type_swap A b : forall a1 a2 : A,
   PCperm_Type b (a1 :: a2 :: nil) (a2 :: a1 :: nil).
 Proof.
 destruct b ; intros.
@@ -97,48 +96,47 @@ destruct b ; intros.
 - apply cperm_Type_swap.
 Qed.
 
-Lemma PCperm_Type_last {A} b : forall (a : A) l,
+Lemma PCperm_Type_last A b : forall (a : A) l,
   PCperm_Type b (a :: l) (l ++ a :: nil).
 Proof.
-destruct b ; intros ;
-  rewrite <- (app_nil_l l) ; rewrite app_comm_cons.
+destruct b; intros; rewrite <- (app_nil_l l), app_comm_cons.
 - apply Permutation_Type_cons_append.
 - apply cperm_Type_last.
 Qed.
 
-Lemma PCperm_Type_app_comm {A} b : forall l l',
+Lemma PCperm_Type_app_comm A b : forall l l',
   @PCperm_Type A b (l ++ l') (l' ++ l).
 Proof.
-destruct b ; intros.
+destruct b; intros.
 - apply Permutation_Type_app_comm.
 - apply cperm_Type.
 Qed.
 
-Lemma PCperm_Type_app_rot {A} b : forall l1 l2 l3,
+Lemma PCperm_Type_app_rot A b : forall l1 l2 l3,
   @PCperm_Type A b  (l1 ++ l2 ++ l3) (l2 ++ l3 ++ l1).
 Proof.
-destruct b ; intros.
+destruct b; intros.
 - apply Permutation_Type_app_rot.
 - apply cperm_Type_app_rot.
 Qed.
 
-Lemma PCperm_Type_nil {A} b : forall l,
+Lemma PCperm_Type_nil A b : forall l,
   @PCperm_Type A b nil l -> l = nil.
-Proof with try assumption.
-destruct b ; intros.
-- apply Permutation_Type_nil...
-- apply cperm_Type_nil...
+Proof.
+destruct b; intros.
+- now apply Permutation_Type_nil.
+- now apply cperm_Type_nil.
 Qed.
 
-Lemma PCperm_Type_nil_cons {A} b : forall l (a : A),
+Lemma PCperm_Type_nil_cons A b : forall l (a : A),
   PCperm_Type b nil (a :: l) -> False.
-Proof with try eassumption.
-destruct b ; intros.
-- eapply Permutation_Type_nil_cons...
-- eapply cperm_Type_nil_cons...
+Proof.
+destruct b; intros.
+- now apply Permutation_Type_nil_cons with _ l a.
+- now apply cperm_Type_nil_cons with l a.
 Qed.
 
-Lemma PCperm_Type_length_1_inv {A} b : forall (a : A) l,
+Lemma PCperm_Type_length_1_inv A b : forall (a : A) l,
   PCperm_Type b (a :: nil) l -> l = a :: nil.
 Proof with try assumption.
 destruct b ; intros.
@@ -146,7 +144,7 @@ destruct b ; intros.
 - apply cperm_Type_one_inv...
 Qed.
 
-Lemma PCperm_Type_length_2_inv {A} b : forall (a1 : A) a2 l,
+Lemma PCperm_Type_length_2_inv A b : forall (a1 : A) a2 l,
   PCperm_Type b (a1 :: a2 :: nil) l -> { l = a1 :: a2 :: nil } + { l = a2 :: a1 :: nil }.
 Proof with try assumption.
 destruct b ; intros.
@@ -154,7 +152,7 @@ destruct b ; intros.
 - apply cperm_Type_two_inv...
 Qed.
 
-Lemma PCperm_Type_vs_elt_inv {A} b : forall (a : A) l l1 l2,
+Lemma PCperm_Type_vs_elt_inv A b : forall (a : A) l l1 l2,
   PCperm_Type b l (l1 ++ a :: l2) ->
   {' (l1',l2') : _ & l = l1' ++ a :: l2' & PEperm_Type b (l2 ++ l1) (l2' ++ l1') }.
 Proof with try reflexivity.
@@ -175,7 +173,7 @@ destruct b ; intros a l l1 l2 HC.
   assumption.
 Qed.
 
-Lemma PCperm_Type_vs_cons_inv {A} b : forall (a : A) l l1,
+Lemma PCperm_Type_vs_cons_inv A b : forall (a : A) l l1,
   PCperm_Type b l (a :: l1) ->
   {' (l1',l2') : _ & l = l1' ++ a :: l2' & PEperm_Type b l1 (l2' ++ l1') }.
 Proof with try reflexivity.
@@ -188,95 +186,90 @@ rewrite app_nil_r in Heq.
 assumption.
 Qed.
 
-Lemma PCperm_Type_cons_vs_cons {A} B : forall (a b : A) la lb,
+Lemma PCperm_Type_cons_vs_cons A B : forall (a b : A) la lb,
   PCperm_Type B (b :: lb) (a :: la) ->
     ( prod (a = b) (PEperm_Type B lb la) )
   + { '(l1,l2) : _ & lb = l1 ++ a :: l2 & PEperm_Type B la (l2 ++ b :: l1) }.
-Proof with try reflexivity.
+Proof.
 intros a b l1 l2 HP.
 apply PCperm_Type_vs_cons_inv in HP.
 destruct HP as [(l1',l2') Heq HP'].
 destruct l1' ; inversion Heq ; subst.
-- left.
-  split.
-  + reflexivity.
-  + rewrite app_nil_r in HP'.
-    destruct B; symmetry; apply HP'.
-- right.
-  exists (l1', l2').
-  + reflexivity.
-  + assumption.
+- left; split; auto.
+  rewrite app_nil_r in HP'.
+  destruct B; symmetry; apply HP'.
+- right; exists (l1', l2'); auto.
 Qed.
 
-Instance PCperm_Type_map {A B} (f : A -> B) b :
+Instance PCperm_Type_map A B (f : A -> B) b :
   Proper (PCperm_Type b ==> PCperm_Type b) (map f).
-Proof with try assumption.
-destruct b ; intros l1 l2 HC.
-- apply Permutation_Type_map...
-- apply cperm_Type_map...
+Proof.
+destruct b; intros l1 l2 HC.
+- now apply Permutation_Type_map.
+- now apply cperm_Type_map.
 Qed.
 
-Lemma PCperm_Type_map_inv {A B} b : forall (f : A -> B) l1 l2,
+Lemma PCperm_Type_map_inv A B b : forall (f : A -> B) l1 l2,
   PCperm_Type b l1 (map f l2) ->
   { l : _ & l1 = map f l & (PCperm_Type b l2 l) }.
 Proof.
-destruct b ; intros.
-- eapply Permutation_Type_map_inv ; eassumption.
-- eapply cperm_Type_map_inv ; eassumption.
+destruct b; intros.
+- now apply Permutation_Type_map_inv.
+- now apply cperm_Type_map_inv.
 Qed.
 
-Instance PCperm_Type_in {A} b (a : A) : Proper (PCperm_Type b ==> Basics.impl) (In a).
-Proof with try eassumption.
-destruct b ; intros l l' HP HIn.
-- eapply Permutation_Type_in...
-- eapply cperm_Type_in...
+Instance PCperm_Type_in A b (a : A) : Proper (PCperm_Type b ==> Basics.impl) (In a).
+Proof.
+destruct b; intros l l' HP HIn.
+- now apply Permutation_Type_in with l.
+- now apply cperm_Type_in with l.
 Qed.
 
-Instance PCperm_Type_Forall {A} b (P : A -> Prop) :
+Instance PCperm_Type_Forall A b (P : A -> Prop) :
   Proper (PCperm_Type b ==> Basics.impl) (Forall P).
-Proof with try eassumption.
-destruct b ; intros l1 l2 HP HF.
-- eapply Permutation_Type_Forall...
-- eapply cperm_Type_Forall...
+Proof.
+destruct b; intros l1 l2 HP HF.
+- now apply Permutation_Type_Forall with l1.
+- now apply cperm_Type_Forall with l1.
 Qed.
 
-Instance PCperm_Type_Exists {A} b (P : A -> Prop) :
+Instance PCperm_Type_Exists A b (P : A -> Prop) :
   Proper (PCperm_Type b ==> Basics.impl) (Exists P).
-Proof with try eassumption.
-destruct b ; intros l1 l2 HP HE.
-- eapply Permutation_Type_Exists...
-- eapply cperm_Type_Exists...
+Proof.
+destruct b; intros l1 l2 HP HE.
+- now apply Permutation_Type_Exists with l1.
+- now apply cperm_Type_Exists with l1.
 Qed.
 
-Lemma PCperm_Type_Forall2 {A B} b (P : A -> B -> Type) :
+Lemma PCperm_Type_Forall2 A B b (P : A -> B -> Type) :
   forall l1 l1' l2, PCperm_Type b l1 l1' -> Forall2_inf P l1 l2 ->
     { l2' : _ & PCperm_Type b l2 l2' & Forall2_inf P l1' l2' }.
 Proof.
-destruct b ; [ apply Permutation_Type_Forall2 | apply cperm_Type_Forall2 ].
+destruct b; [ apply Permutation_Type_Forall2 | apply cperm_Type_Forall2 ].
 Qed.
 
-Lemma PCperm_Type_image {A B} b : forall (f : A -> B) a l l',
+Lemma PCperm_Type_image A B b : forall (f : A -> B) a l l',
   PCperm_Type b (a :: l) (map f l') -> { a' | a = f a' }.
-Proof with try eassumption.
-destruct b ; intros.
-- eapply Permutation_Type_image...
-- eapply cperm_Type_image...
+Proof.
+destruct b; intros.
+- now apply Permutation_Type_image with l l'.
+- now apply cperm_Type_image with l l'.
 Qed.
 
-Instance PCperm_Type_Forall_Type {A} b (P : A -> Type) :
+Instance PCperm_Type_Forall_Type A b (P : A -> Type) :
   Proper (PCperm_Type b ==> Basics.arrow) (Forall_inf P).
-Proof with try eassumption.
-destruct b ; intros l1 l2 HP HF.
-- eapply Permutation_Type_Forall_Type...
-- eapply cperm_Type_Forall_Type...
+Proof.
+destruct b; intros l1 l2 HP HF.
+- now apply Permutation_Type_Forall_Type with l1.
+- now apply cperm_Type_Forall_Type with l1.
 Qed.
 
-Instance PCperm_Type_Exists_Type {A} b (P : A -> Type) :
+Instance PCperm_Type_Exists_Type A b (P : A -> Type) :
   Proper (PCperm_Type b ==> Basics.arrow) (Exists_inf P).
-Proof with try eassumption.
-destruct b ; intros l1 l2 HP HE.
-- eapply Permutation_Type_Exists_Type...
-- eapply cperm_Type_Exists_Type...
+Proof.
+destruct b; intros l1 l2 HP HE.
+- now apply Permutation_Type_Exists_Type with l1.
+- now apply cperm_Type_Exists_Type with l1.
 Qed.
 
 
@@ -302,12 +295,10 @@ Ltac PEperm_Type_solve :=
 
 (** *** Properties *)
 
-Instance PEperm_perm_Type {A} b : Proper (PEperm_Type b ==> (@Permutation_Type A)) id.
-Proof.
-destruct b ; intros l l' HP ; simpl in HP ; now subst.
-Qed.
+Instance PEperm_perm_Type A b : Proper (PEperm_Type b ==> (@Permutation_Type A)) id.
+Proof. destruct b; intros l l' HP; simpl in HP; now subst. Qed.
 
-Lemma PEperm_Type_monot {A} : forall b1 b2, Bool.leb b1 b2 ->
+Lemma PEperm_Type_monot A : forall b1 b2, Bool.leb b1 b2 ->
   forall l1 l2 : list A, PEperm_Type b1 l1 l2 -> PEperm_Type b2 l1 l2.
 Proof.
 intros b1 b2 Hleb l1 l2.
@@ -315,28 +306,28 @@ destruct b1; destruct b2; try (now inversion Hleb).
 simpl; intros HP; subst; reflexivity.
 Qed.
 
-Instance PEperm_Type_refl {A} b : Reflexive (@PEperm_Type A b).
+Instance PEperm_Type_refl A b : Reflexive (@PEperm_Type A b).
 Proof.
 destruct b ; intros l.
 - apply Permutation_Type_refl.
 - reflexivity.
 Qed.
 
-Instance PEperm_Type_sym {A} b : Symmetric (@PEperm_Type A b).
-Proof with try assumption.
+Instance PEperm_Type_sym A b : Symmetric (@PEperm_Type A b).
+Proof.
 destruct b ; intros l l' HP.
-- apply Permutation_Type_sym...
-- symmetry...
+- now apply Permutation_Type_sym.
+- now symmetry.
 Qed.
 
-Instance PEperm_Type_trans {A} b : Transitive (@PEperm_Type A b).
-Proof with try eassumption.
-destruct b ; intros l l' l'' HP1 HP2.
-- eapply Permutation_Type_trans...
-- etransitivity...
+Instance PEperm_Type_trans A b : Transitive (@PEperm_Type A b).
+Proof.
+destruct b; intros l l' l'' HP1 HP2.
+- now apply Permutation_Type_trans with l'.
+- now transitivity l'.
 Qed.
 
-Instance PEperm_Type_equiv {A} b : Equivalence (@PEperm_Type A b).
+Instance PEperm_Type_equiv A b : Equivalence (@PEperm_Type A b).
 Proof.
 split.
 - apply PEperm_Type_refl.
@@ -344,14 +335,14 @@ split.
 - apply PEperm_Type_trans.
 Qed.
 
-Instance eq_PEperm_Type {A} b : Proper (eq ==> PEperm_Type b) (@id (list A)).
+Instance eq_PEperm_Type A b : Proper (eq ==> PEperm_Type b) (@id (list A)).
 Proof.
-destruct b ; intros l l' Heq ; subst.
+destruct b; intros l l' Heq; subst.
 - apply Permutation_Type_refl.
 - reflexivity.
 Qed.
 
-Instance PEperm_Type_cons {A} b :
+Instance PEperm_Type_cons A b :
   Proper (eq ==> PEperm_Type b ==> PEperm_Type b) (@cons A).
 Proof.
 destruct b ; intros x y Heq l1 l2 HP ; subst.
@@ -359,14 +350,14 @@ destruct b ; intros x y Heq l1 l2 HP ; subst.
 - now rewrite HP.
 Qed.
 
-Instance PEperm_Type_app {A} b : Proper (PEperm_Type b ==> PEperm_Type b ==> PEperm_Type b) (@app A).
+Instance PEperm_Type_app A b : Proper (PEperm_Type b ==> PEperm_Type b ==> PEperm_Type b) (@app A).
 Proof.
 destruct b ; simpl ; intros l m HP1 l' m' HP2.
 - now apply Permutation_Type_app.
 - now subst.
 Qed.
 
-Lemma PEperm_Type_app_tail {A} b : forall l l' tl : list A,
+Lemma PEperm_Type_app_tail A b : forall l l' tl : list A,
   PEperm_Type b l l' -> PEperm_Type b (l ++ tl) (l' ++ tl).
 Proof.
 destruct b ; simpl ; intros l l' tl HP.
@@ -374,7 +365,7 @@ destruct b ; simpl ; intros l l' tl HP.
 - now subst.
 Qed.
 
-Lemma PEperm_Type_app_head {A} b : forall l tl tl' : list A,
+Lemma PEperm_Type_app_head A b : forall l tl tl' : list A,
   PEperm_Type b tl tl' -> PEperm_Type b (l ++ tl) (l ++ tl').
 Proof.
 destruct b ; simpl ; intros l tl tl' HP.
@@ -382,7 +373,7 @@ destruct b ; simpl ; intros l tl tl' HP.
 - now subst.
 Qed.
 
-Lemma PEperm_Type_add_inside {A} b : forall (a : A) l l' tl tl',
+Lemma PEperm_Type_add_inside A b : forall (a : A) l l' tl tl',
   PEperm_Type b l l' -> PEperm_Type b tl tl' -> PEperm_Type b (l ++ a :: tl) (l' ++ a :: tl').
 Proof.
 destruct b ; simpl ; intros a l l' tl tl' HP1 HP2.
@@ -390,166 +381,151 @@ destruct b ; simpl ; intros a l l' tl tl' HP1 HP2.
 - now subst.
 Qed.
 
-Lemma PEperm_Type_nil {A} b : forall l, @PEperm_Type A b nil l -> l = nil.
-Proof with try assumption.
-destruct b ; intros.
-- apply Permutation_Type_nil...
-- symmetry...
+Lemma PEperm_Type_nil A b : forall l, @PEperm_Type A b nil l -> l = nil.
+Proof.
+destruct b; intros.
+- now apply Permutation_Type_nil.
+- now symmetry.
 Qed.
 
-Lemma PEperm_nil_cons {A} b : forall l (a : A),
+Lemma PEperm_nil_cons A b : forall l (a : A),
   PEperm_Type b nil (a :: l) -> False.
-Proof with try eassumption.
-destruct b ; intros l a H.
-- eapply Permutation_Type_nil_cons...
+Proof.
+destruct b; intros l a H.
+- now apply Permutation_Type_nil_cons with _ l a.
 - inversion H.
 Qed.
 
-Lemma PEperm_Type_length_1_inv {A} b : forall (a : A) l,
+Lemma PEperm_Type_length_1_inv A b : forall (a : A) l,
   PEperm_Type b (a :: nil) l -> l = a :: nil.
-Proof with try assumption.
-destruct b ; intros.
-- apply Permutation_Type_length_1_inv...
-- symmetry...
+Proof.
+destruct b; intros.
+- now apply Permutation_Type_length_1_inv.
+- now symmetry.
 Qed.
 
-Lemma PEperm_Type_length_2_inv {A} b : forall (a1 : A) a2 l,
+Lemma PEperm_Type_length_2_inv A b : forall (a1 : A) a2 l,
   PEperm_Type b (a1 :: a2 :: nil) l -> { l = a1 :: a2 :: nil } + { l = a2 :: a1 :: nil }.
-Proof with try assumption.
-destruct b ; intros.
-- apply Permutation_Type_length_2_inv...
-- left ; symmetry...
+Proof.
+destruct b; intros.
+- now apply Permutation_Type_length_2_inv.
+- now left; symmetry.
 Qed.
 
-Lemma PEperm_Type_vs_elt_inv {A} b : forall (a : A) l l1 l2,
+Lemma PEperm_Type_vs_elt_inv A b : forall (a : A) l l1 l2,
   PEperm_Type b l (l1 ++ a :: l2) ->
-  {'(l1', l2') : _ & l = l1' ++ a :: l2' & PEperm_Type b (l1 ++ l2) (l1' ++ l2') }.
-Proof with try reflexivity.
-destruct b ; simpl ; intros a l l1 l2 HP.
-- assert (HP' := HP).
-  apply Permutation_Type_vs_elt_inv in HP'.
-  destruct HP' as ((l',l'') & Heq) ; subst.
-  apply Permutation_Type_app_inv in HP.
-  apply Permutation_Type_sym in HP.
-  exists (l',l'')...
-  assumption.
-- subst.
-  exists (l1,l2)...
+  {'(l1', l2') & l = l1' ++ a :: l2' & PEperm_Type b (l1 ++ l2) (l1' ++ l2') }.
+Proof.
+destruct b; simpl; intros a l l1 l2 HP; subst.
+- destruct (Permutation_Type_vs_elt_inv _ _ _ _ HP) as ((l',l'') & Heq) ; subst.
+  apply Permutation_Type_app_inv, Permutation_Type_sym in HP.
+  now exists (l', l'').
+- now exists (l1, l2).
 Qed.
 
-Lemma PEperm_Type_vs_cons_inv {A} b : forall (a : A) l l1,
+Lemma PEperm_Type_vs_cons_inv A b : forall (a : A) l l1,
   PEperm_Type b l (a :: l1) ->
   {'(l1', l2') : _ & l = l1' ++ a :: l2' & PEperm_Type b l1 (l1' ++ l2') }.
 Proof.
 intros a l l1 HP.
 rewrite <- (app_nil_l l1).
-eapply PEperm_Type_vs_elt_inv.
-assumption.
+now apply PEperm_Type_vs_elt_inv.
 Qed.
 
-Instance PEperm_Type_in {A} b (a : A) : Proper (PEperm_Type b ==> Basics.impl) (In a).
-Proof with try eassumption.
-destruct b ; simpl ; intros l l' HP HIn.
-- eapply Permutation_Type_in...
-- subst...
+Instance PEperm_Type_in A b (a : A) : Proper (PEperm_Type b ==> Basics.impl) (In a).
+Proof.
+destruct b; simpl; intros l l' HP HIn; subst; auto.
+now apply Permutation_Type_in with l.
 Qed.
 
-Instance PEperm_Type_Forall {A} b (P : A -> Prop) :
+Instance PEperm_Type_Forall A b (P : A -> Prop) :
   Proper (PEperm_Type b ==> Basics.impl) (Forall P).
-Proof with try eassumption.
-destruct b ; simpl ; intros l1 l2 HP HF.
-- eapply Permutation_Type_Forall...
-- subst...
+Proof.
+destruct b; simpl; intros l1 l2 HP HF; subst; auto.
+now apply Permutation_Type_Forall with l1.
 Qed.
 
-Instance PEperm_Type_Exists {A} b (P : A -> Prop) :
+Instance PEperm_Type_Exists A b (P : A -> Prop) :
   Proper (PEperm_Type b ==> Basics.impl) (Exists P).
-Proof with try eassumption.
-destruct b ; simpl ; intros l1 l2 HP HF.
-- eapply Permutation_Type_Exists...
-- subst...
+Proof.
+destruct b; simpl; intros l1 l2 HP HF; subst; auto.
+now apply Permutation_Type_Exists with l1.
 Qed.
 
-Lemma PEperm_Type_Forall2 {A B} b (P : A -> B -> Prop) :
+Lemma PEperm_Type_Forall2 A B b (P : A -> B -> Prop) :
   forall l1 l1' l2, PEperm_Type b l1 l1' -> Forall2_inf P l1 l2 ->
     { l2' : _ & PEperm_Type b l2 l2' & Forall2_inf P l1' l2' }.
 Proof.
-destruct b ; [ apply Permutation_Type_Forall2 | ].
-intros l1 l1' l2 HE HF ; simpl in HE ; subst.
-exists l2 ; [ reflexivity | assumption ].
+destruct b; [ apply Permutation_Type_Forall2 | ].
+intros l1 l1' l2 HE HF; simpl in HE; subst.
+now exists l2.
 Qed.
 
-Instance PEperm_Type_map {A B} (f : A -> B) b :
+Instance PEperm_Type_map A B (f : A -> B) b :
   Proper (PEperm_Type b ==> PEperm_Type b) (map f).
 Proof.
-destruct b ; intros l l' HP.
-- apply Permutation_Type_map.
-  assumption.
-- simpl in HP ; subst.
-  reflexivity.
+destruct b; intros l l' HP; simpl in HP; subst.
+- now apply Permutation_Type_map.
+- reflexivity.
 Qed.
 
-Instance PEperm_Type_Forall_Type {A} b (P : A -> Type) :
+Instance PEperm_Type_Forall_Type A b (P : A -> Type) :
   Proper (PEperm_Type b ==> Basics.arrow) (Forall_inf P).
-Proof with try eassumption.
-destruct b ; simpl ; intros l1 l2 HP HF.
-- eapply Permutation_Type_Forall_Type...
-- subst...
+Proof.
+destruct b; simpl; intros l1 l2 HP HF; subst; auto.
+now apply Permutation_Type_Forall_Type with l1.
 Qed.
 
-Instance PEperm_Type_Exists_Type {A} b (P : A -> Type) :
+Instance PEperm_Type_Exists_Type A b (P : A -> Type) :
   Proper (PEperm_Type b ==> Basics.arrow) (Exists_inf P).
-Proof with try eassumption.
-destruct b ; simpl ; intros l1 l2 HP HF.
-- eapply Permutation_Type_Exists_Type...
-- subst...
+Proof.
+destruct b; simpl; intros l1 l2 HP HF; subst; auto.
+now apply Permutation_Type_Exists_Type with l1.
 Qed.
 
-Lemma PEperm_Type_map_inv {A B} b : forall (f : A -> B) l1 l2,
+Lemma PEperm_Type_map_inv A B b : forall (f : A -> B) l1 l2,
   PEperm_Type b l1 (map f l2) ->
   { l : _ & l1 = map f l & (PEperm_Type b l2 l) }.
 Proof.
-destruct b ; simpl ; intros f l1 l2 HP.
-- eapply Permutation_Type_map_inv ; eassumption.
-- subst.
-  exists l2 ; reflexivity.
+destruct b; simpl; intros f l1 l2 HP.
+- now apply Permutation_Type_map_inv.
+- now subst; exists l2.
 Qed.
 
-Instance PEperm_Type_rev {A} b : Proper (PEperm_Type b ==> PEperm_Type b) (@rev A).
+Instance PEperm_Type_rev A b : Proper (PEperm_Type b ==> PEperm_Type b) (@rev A).
 Proof.
 destruct b ; intros l1 l2 HP.
 - now apply Permutation_Type_rev'.
 - now (simpl in HP ; subst).
 Qed.
 
-Lemma PEperm_Type_map_inv_inj {A B} b : forall f : A -> B, injective f ->
+Lemma PEperm_Type_map_inv_inj A B b : forall f : A -> B, injective f ->
   forall l1 l2, PEperm_Type b (map f l1) (map f l2) -> PEperm_Type b l1 l2.
-Proof with try assumption.
-destruct b ; intros f Hi l1 l2 HP.
-- apply Permutation_Type_map_inv_inj in HP...
-- apply map_injective in HP...
+Proof.
+destruct b; intros f Hi l1 l2 HP.
+- now apply Permutation_Type_map_inv_inj in HP.
+- now apply map_injective in HP.
 Qed.
 
-Lemma PEperm_Type_image {A B} b : forall (f : A -> B) a l l',
+Lemma PEperm_Type_image A B b : forall (f : A -> B) a l l',
   PEperm_Type b (a :: l) (map f l') -> { a' | a = f a' }.
 Proof.
 destruct b ; intros f a l l' H.
-- eapply Permutation_Type_image ; eassumption.
-- destruct l' ; inversion H ; subst.
-  exists a0 ; reflexivity.
+- now apply Permutation_Type_image with l l'.
+- destruct l'; inversion H; subst.
+  now exists a0.
 Qed.
 
 
 (** ** From PEperm to PCperm *)
 
-Instance PEperm_PCperm_Type {A} b : Proper (PEperm_Type b ==> PCperm_Type b) (@id (list A)).
+Instance PEperm_PCperm_Type A b : Proper (PEperm_Type b ==> PCperm_Type b) (@id (list A)).
 Proof.
-destruct b ; simpl ; intros l l' HP.
-- assumption.
-- subst ; apply cperm_Type_refl.
+destruct b; simpl; intros l l' HP; auto.
+subst ; apply cperm_Type_refl.
 Qed.
 
-Instance PEperm_PCperm_Type_cons {A} b :
+Instance PEperm_PCperm_Type_cons A b :
   Proper (eq ==> PEperm_Type b ==> PCperm_Type b) (@cons A).
 Proof.
 intros x y Heq l1 l2 HP ; subst.
@@ -557,12 +533,10 @@ apply PEperm_PCperm_Type.
 now apply PEperm_Type_cons.
 Qed.
 
-Instance PEperm_PCperm_Type_app {A} b :
+Instance PEperm_PCperm_Type_app A b :
   Proper (PEperm_Type b ==> PEperm_Type b ==> PCperm_Type b) (@app A).
 Proof.
 intros l1 l1' HPhd l2 l2' HPtl.
 apply PEperm_PCperm_Type.
-rewrite HPhd.
-rewrite HPtl.
-reflexivity.
+now rewrite HPhd, HPtl.
 Qed.
