wf_prod.v
@@ -1,39 +1,36 @@
-(* wf_prod Library *)
-
 (** * Well-founded order on product and applications to products of nat *)
 
 Require Import Relation_Definitions Wf_nat Lia.
 
+Set Implicit Arguments.
 
 (** * Non-Dependant Product of two [well_founded] relations *)
 
 Section Product.
 
-Variable A B : Type.
-Variable RA : relation A.
-Variable RB : relation B.
-Hypothesis WA : well_founded RA.
-Hypothesis WB : well_founded RB.
+  Variable A B : Type.
+  Variable RA : relation A.
+  Variable RB : relation B.
+  Hypothesis WA : well_founded RA.
+  Hypothesis WB : well_founded RB.
 
-(* more general but slightly different type
-Definition lt_prod v1 v2 := lexprod _ _ RA (fun _ => RB) v1 v2.
-Definition wf_prod := wf_lexprod _ _ _ _ WA (fun _ => WB).
-*)
-Definition lt_prod v1 v2 := RA (fst v1) (fst v2)
-     \/ (fst v1 = fst v2 /\ RB (snd v1) (snd v2)).
+  (* more general but slightly different type
+  Definition lt_prod v1 v2 := lexprod _ _ RA (fun _ => RB) v1 v2.
+  Definition wf_prod := wf_lexprod _ _ _ _ WA (fun _ => WB).
+  *)
+  Definition lt_prod v1 v2 := RA (fst v1) (fst v2)
+       \/ (fst v1 = fst v2 /\ RB (snd v1) (snd v2)).
 
-Lemma wf_prod : well_founded lt_prod.
-Proof with assumption.
-intros [a b].
-revert b.
-induction a using (well_founded_induction WA) ;
-induction b using (well_founded_induction WB).
-constructor.
-intros [a' b'] [Ho | [L R]].
-- apply H...
-- simpl in L ; subst.
-  apply H0...
-Qed.
+  Lemma wf_prod : well_founded lt_prod.
+  Proof.
+  intros [a b]; revert b.
+  induction a using (well_founded_induction WA);
+    induction b using (well_founded_induction WB).
+  constructor.
+  intros [a' b'] [Ho | [L R]].
+  - now apply H.
+  - now simpl in L; subst; apply H0.
+  Qed.
 
 End Product.
 
@@ -44,8 +41,8 @@ End Product.
 Definition lt_nat_nat := lexprod _ _ lt (fun _ => lt).
 Definition wf_nat_nat := wf_lexprod _ _ _ _ lt_wf (fun _ => lt_wf).
 *)
-Definition lt_nat_nat := lt_prod _ _ lt lt.
-Definition wf_nat_nat := wf_prod _ _ _ _ lt_wf lt_wf.
+Definition lt_nat_nat := lt_prod lt lt.
+Definition wf_nat_nat := wf_prod lt_wf lt_wf.
 
 Ltac lt_nat_nat_solve :=
   match goal with
@@ -59,8 +56,8 @@ Ltac lt_nat_nat_solve :=
 
 (** * Well founded order on triples of [nat] *)
 
-Definition lt_nat_nat_nat := lt_prod _ _ lt lt_nat_nat.
-Definition wf_nat_nat_nat := wf_prod _ _ _ _ lt_wf wf_nat_nat.
+Definition lt_nat_nat_nat := lt_prod lt lt_nat_nat.
+Definition wf_nat_nat_nat := wf_prod lt_wf wf_nat_nat.
 
 Ltac lt_nat_nat_nat_solve :=
   match goal with 
@@ -80,4 +77,3 @@ Ltac lt_nat_nat_nat_solve :=
      try (right; split; [ | right; split ]; simpl; lia);
      fail
   end.
-
